refactor: use Program instead of refine

src/x86/Architecture/MemoryController/Registers/Smramc_eq.v
@@ -1,27 +1,40 @@
+Require Import Coq.Program.Tactics.
+
 Require Import Coq.Bool.Sumbool.
 Require Import Coq.Bool.Bool.
 
 Require Import SpecCert.Utils.
 Require Import SpecCert.x86.Architecture.MemoryController.Registers.Smramc_rec.
 
-Definition smramc_eq (s s':SmramcRegister) :=
+Definition smramc_eq
+           (s s': SmramcRegister) :=
   d_open s = d_open s' /\ d_lock s = d_lock s'.
 
-Axiom smramc_eq_eq: forall s s':SmramcRegister,
-  smramc_eq s s' -> s = s'.
+Axiom smramc_eq_eq:
+  forall s s':SmramcRegister,
+    smramc_eq s s' -> s = s'.
 
-Axiom eq_smramc_eq: forall s s':SmramcRegister,
-  s = s' -> smramc_eq s s'.
+Axiom eq_smramc_eq:
+  forall s s':SmramcRegister,
+    s = s'
+    -> smramc_eq s s'.
 
-Definition smramc_eq_dec (s s':SmramcRegister): {smramc_eq s s'}+{~smramc_eq s s'}.
-  refine (
-    let o := d_open s in
-    let o' := d_open s' in
-    let l := d_lock s in
-    let l' := d_lock s' in
-      decide_dec (sumbool_and _ _ _ _  (bool_dec o o') (bool_dec l l'))
-  ); firstorder.
+Program Definition smramc_eq_dec
+        (s s': SmramcRegister)
+  : { smramc_eq s s' } + { ~ smramc_eq s s' } :=
+  let o := d_open s in
+  let o' := d_open s' in
+  let l := d_lock s in
+  let l' := d_lock s' in
+  (bool_dec o o') :&& (bool_dec l l').
+Next Obligation.
+  unfold smramc_eq.
+  split; [exact H|exact H0].
 Qed.
-
-Definition smramc_eqb (s s':SmramcRegister) :=
-  if smramc_eq_dec s s' then true else false.
+Next Obligation.
+  unfold smramc_eq.
+  destruct H as [H|H];
+    intros [H' H'']; [ apply H in H'; exact H'
+                     | apply H in H''; exact H''
+                     ].
+Qed.
