src/Utils.v
@@ -1,6 +1,10 @@
+Require Import Coq.Bool.Sumbool.
+
 Notation "'true_dec'" := (left _ _).
 Notation "'false_dec'" := (right _ _).
 Notation "'decide_dec' x" := (if x then
     true_dec
   else
     false_dec) (at level 42).
+Notation "x :&& y" := (decide_dec (sumbool_and _ _ _ _ x y)) (at level 42).
+Notation "x :|| y" := (decide_dec (sumbool_or _ _ _ _ x y)) (at level 42).
