src/x86/Architecture/MemoryController/MemoryController_dec.v
@@ -1,5 +1,5 @@
+Require Import Coq.Program.Tactics.
 Require Import Coq.Bool.Bool.
-Require Import Coq.Bool.Sumbool.
 
 Require Import SpecCert.Utils.
 Require Import SpecCert.x86.Architecture.MemoryController.MemoryController_rec.
@@ -7,27 +7,23 @@ Require Import SpecCert.x86.Architecture.MemoryController.MemoryController_prop.
 Require Import SpecCert.x86.Architecture.MemoryController.Registers.
 
 Definition smramc_is_locked_dec
-           (mc :MemoryController)
-           :{smramc_is_locked mc}+{~smramc_is_locked mc}.
-refine (
-  decide_dec (smramc_is_ro_dec (smramc mc))
-); unfold smramc_is_locked; trivial.
-Defined.
+           (mc: MemoryController)
+  : { smramc_is_locked mc } + { ~ smramc_is_locked mc } :=
+  smramc_is_ro_dec (smramc mc).
 
 Definition smramc_is_unlocked_dec
-           (mc :MemoryController)
-           :{smramc_is_unlocked mc}+{~smramc_is_unlocked mc}.
-refine (
-  decide_dec (smramc_is_rw_dec (smramc mc))
-); unfold smramc_is_locked; trivial.
-Defined.
+           (mc: MemoryController)
+  : { smramc_is_unlocked mc } + { ~ smramc_is_unlocked mc } :=
+  smramc_is_rw_dec (smramc mc).
 
-Definition can_access_smram_dec
-           (mc     :MemoryController)
-           (smiact :bool)
-           :{can_access_smram mc smiact}+{~can_access_smram mc smiact}.
-refine (
-  decide_dec (sumbool_or _ _ _ _ (bool_dec smiact true)
-                                 (bool_dec (d_open (smramc mc)) true))
-); firstorder.
+Program Definition can_access_smram_dec
+        (mc:     MemoryController)
+        (smiact: bool)
+  : { can_access_smram mc smiact } + { ~ can_access_smram mc smiact } :=
+  (bool_dec smiact true) :|| (bool_dec (d_open (smramc mc)) true).
+Next Obligation.
+  unfold can_access_smram.
+  intros [H'|H'].
+  + apply H in H'; exact H'.
+  + apply H0 in H'; exact H'.
 Qed.
