src/x86/Architecture/ProcessorUnit/ProcessorUnit_dec.v
@@ -8,55 +8,57 @@ Require Import SpecCert.x86.Architecture.ProcessorUnit.ProcessorUnit_prop.
 Require Import SpecCert.Address.
 Require Import SpecCert.Interval.
 
-Definition interrupts_are_disabled_dec (p:ProcessorUnit)
-  : {interrupts_are_disabled p}+{~interrupts_are_disabled p}.
-refine (
-  decide_dec (bool_dec (cli p) true)
-); trivial.
-Defined.
+Definition interrupts_are_disabled_dec
+           (p: ProcessorUnit)
+  : { interrupts_are_disabled p } + { ~ interrupts_are_disabled p } :=
+  bool_dec (cli p) true.
 
-Definition interrupts_are_enabled_dec (p:ProcessorUnit)
-  : {interrupts_are_enabled p}+{~interrupts_are_enabled p}.
-refine (
-  decide_dec (bool_dec (cli p) false)
-  ); trivial.
-Defined.
+Definition interrupts_are_enabled_dec
+           (p: ProcessorUnit)
+  : { interrupts_are_enabled p } + { ~ interrupts_are_enabled p } :=
+  bool_dec (cli p) false.
 
-Definition will_process_interrupt_dec (p:ProcessorUnit)(i:Interrupt)
-  : {will_process_interrupt p i}+{~will_process_interrupt p i}.
-refine (
-  decide_dec (sumbool_or _ _ _ _ (interrupt_eq_dec i SMI)
-                                 (interrupts_are_enabled_dec p))
-  ); unfold will_process_interrupt; trivial.
-apply and_not_or; trivial.
-Defined.
+Program Definition will_process_interrupt_dec
+        (p: ProcessorUnit)
+        (i: Interrupt)
+  : { will_process_interrupt p i } + { ~ will_process_interrupt p i } :=
+  (interrupt_eq_dec i SMI) :|| (interrupts_are_enabled_dec p).
+Next Obligation.
+  unfold will_process_interrupt.
+  intros [Hsmi|Henable].
+  + apply H in Hsmi.
+    exact Hsmi.
+  + apply H0 in Henable.
+    exact Henable.
+Qed.
 
-Definition is_in_smm_dec (p:ProcessorUnit): {is_in_smm p}+{~is_in_smm p}.
-refine (
-    decide_dec (bool_dec (in_smm p) true)
-  ); trivial.
-Defined.  
+Definition is_in_smm_dec
+           (p: ProcessorUnit)
+  : { is_in_smm p } + { ~ is_in_smm p } :=
+    bool_dec (in_smm p) true.
 
-Definition is_inside_smrr_dec (p:ProcessorUnit)(pa:PhysicalAddress)
-  :{is_inside_smrr p pa}+{~is_inside_smrr p pa}.
-refine (
-    decide_dec (is_inside_interval_dec (address_offset pa)
-                                       (interval (smrr p))
-               )
-  ); intuition.
-Defined.
+Definition is_inside_smrr_dec
+           (p:  ProcessorUnit)
+           (pa: PhysicalAddress)
+  : { is_inside_smrr p pa } + { ~ is_inside_smrr p pa } :=
+    is_inside_interval_dec (address_offset pa)
+                           (interval (smrr p)).
 
-Definition smrr_hit_dec
-           (p:ProcessorUnit)
-           (pa:PhysicalAddress)
-  : {smrr_hit p pa} + {~ smrr_hit p pa}.
-refine (
-    decide_dec (sumbool_and _ _ _ _
-                            (is_in_smm_dec p)
-                            (is_inside_smrr_dec p pa)
-               )
-  ); trivial.
-unfold smrr_hit.
-apply or_not_and.
-trivial.
-Defined.
+Program Definition smrr_hit_dec
+        (p:  ProcessorUnit)
+        (pa: PhysicalAddress)
+  : { smrr_hit p pa } + { ~ smrr_hit p pa } :=
+  (is_in_smm_dec p) :&& (is_inside_smrr_dec p pa).
+Next Obligation.
+  unfold smrr_hit.
+  split; [exact H|exact H0].
+Qed.
+Next Obligation.
+  unfold smrr_hit.
+  intros [Hsmm Hinside].
+  destruct H as [H|H]; [ apply H in Hsmm;
+                         exact Hsmm
+                       | apply H in Hinside;
+                         exact Hinside
+                       ].
+Qed.
